

Since I have already taken the midterm, I will only be completing the exercises related to the second part of the course (from differential kinematics onwards).

#### Exercise 4

The kinematics of a 4-dof robot manipulator is characterized by the DH parameters in Tab. 1. Build the geometric Jacobian  $J(q)$  that relates the joint velocities  $\dot{q} \in \mathbb{R}^4$  to the six-dimensional twist vector composed by a velocity  $v = v_4 \in \mathbb{R}^3$  of the origin of the last (end-effector) DH frame and by an angular velocity  $\omega = \omega_4 \in \mathbb{R}^3$  of the same frame:

$$\begin{pmatrix} v \\ \omega \end{pmatrix} = J(q)\dot{q}.$$

$i$	$\alpha_i$	$a_i$	$d_i$	$\theta_i$
1	$\pi/2$	0	0	$q_1$
2	$\pi/2$	0	0	$q_2$
3	$-\pi/2$	0	$q_3$	0
4	0	$a_4$	0	$q_4$

I have to compute the homogeneous transformations.

$${}^0T_1 = \begin{pmatrix} c_1 & 0 & s_1 & 0 \\ s_1 & 0 & -c_1 & 0 \\ 0 & 1 & 0 & 0 \\ 0 & 0 & 0 & 1 \end{pmatrix} \quad {}^1T_2 = \begin{pmatrix} c_2 & 0 & s_2 & 0 \\ s_2 & 0 & -c_2 & 0 \\ 0 & 1 & 0 & 0 \\ 0 & 0 & 0 & 1 \end{pmatrix} \quad {}^2T_3 = \begin{pmatrix} 1 & 0 & 0 & 0 \\ 0 & 0 & 1 & 0 \\ 0 & -1 & 0 & q_3 \\ 0 & 0 & 0 & 1 \end{pmatrix} \quad {}^3T_4 = \begin{pmatrix} c_4 & -s_4 & 0 & a_4 c_4 \\ s_4 & c_4 & 0 & a_4 s_4 \\ 0 & 0 & 1 & 0 \\ 0 & 0 & 0 & 1 \end{pmatrix}$$

$${}^0T_2 = \begin{pmatrix} c_1 & 0 & s_1 & 0 \\ s_1 & 0 & -c_1 & 0 \\ 0 & 1 & 0 & 0 \\ 0 & 0 & 0 & 1 \end{pmatrix} \begin{pmatrix} c_2 & 0 & s_2 & 0 \\ s_2 & 0 & -c_2 & 0 \\ 0 & 1 & 0 & 0 \\ 0 & 0 & 0 & 1 \end{pmatrix} = \begin{pmatrix} c_1 c_2 & s_1 & c_1 s_2 & 0 \\ s_1 c_2 & -c_1 & s_1 s_2 & 0 \\ s_2 & 0 & -c_2 & 0 \\ 0 & 0 & 0 & 1 \end{pmatrix}$$

$${}^0T_3 = {}^0T_2 {}^2T_3 = \begin{pmatrix} c_1 c_2 & s_1 & c_1 s_2 & 0 \\ s_1 c_2 & -c_1 & s_1 s_2 & 0 \\ s_2 & 0 & -c_2 & 0 \\ 0 & 0 & 0 & 1 \end{pmatrix} \begin{pmatrix} 1 & 0 & 0 & 0 \\ 0 & 0 & 1 & 0 \\ 0 & -1 & 0 & q_3 \\ 0 & 0 & 0 & 1 \end{pmatrix} = \begin{pmatrix} c_1 c_2 & -c_1 s_2 & s_1 & q_3 c_1 s_2 \\ s_1 c_2 & -s_1 s_2 & -c_1 & q_3 s_1 s_2 \\ s_2 & c_2 & 0 & -q_3 c_2 \\ 0 & 0 & 0 & 1 \end{pmatrix}$$

For the complete <sup>position</sup> DK I consider only the last column of  ${}^0T_4$

$$f_p(q) = \begin{pmatrix} c_1 c_2 & -c_1 s_2 & s_1 & q_3 c_1 s_2 \\ s_1 c_2 & -s_1 s_2 & -c_1 & q_3 s_1 s_2 \\ s_2 & c_2 & 0 & -q_3 c_2 \\ 0 & 0 & 0 & 1 \end{pmatrix} \begin{pmatrix} a_4 c_4 \\ a_4 s_4 \\ 0 \\ 1 \end{pmatrix} = \begin{cases} a_4 c_1 c_2 c_4 - a_4 c_1 s_2 s_4 + q_3 c_1 s_2 \\ a_4 s_1 c_2 c_4 - a_4 s_1 s_2 c_4 + q_3 s_1 s_2 \\ a_4 (s_2 c_4 + c_2 s_4) - q_3 c_2 \\ a_4 s_2 s_4 - q_3 c_2 \end{cases} = \begin{cases} c_1 (a_4 c_2 c_4 + q_3 s_2) \\ s_1 (a_4 c_2 c_4 + q_3 s_2) \\ a_4 s_2 c_4 - q_3 c_2 \\ a_4 s_2 s_4 - q_3 c_2 \end{cases} = p_{0,e}$$

I need to compute  $p_{1,e}, p_{2,e}, p_{3,e}, z_1, z_2, z_3$

We recall that  $p_{0,i} = {}^0T_i \cdot (0 \ 0 \ 0 \ 1)^T$  so:

$$p_{1,e} = p_{0,e} - p_{0,1} = p_{1,e} \quad p_{3,e} = p_{0,e} - p_{0,3} = \begin{cases} c_1 a_4 c_2 c_4 \\ s_1 a_4 c_2 c_4 \\ a_4 s_2 c_4 \end{cases} \quad S_3 = \begin{pmatrix} 0 & 0 & -c_1 \\ 0 & 0 & -s_1 \\ c_1 & s_1 & 0 \end{pmatrix}$$

skew symmetric matrices

$$\text{Then: } z_1 = \begin{pmatrix} s_1 \\ -c_1 \\ 0 \end{pmatrix} \quad z_2 = \begin{pmatrix} c_1 s_2 \\ s_1 s_2 \\ -c_2 \end{pmatrix} \quad z_3 = \begin{pmatrix} s_1 \\ -c_1 \\ 0 \end{pmatrix} \Rightarrow S_1 = \begin{pmatrix} 0 & 0 & -c_1 \\ 0 & 0 & -s_1 \\ c_1 & s_1 & 0 \end{pmatrix}, \quad S_2 = \begin{pmatrix} 0 & c_2 & s_1 s_2 \\ -c_2 & 0 & -c_1 s_2 \\ -s_1 s_2 & c_1 s_2 & 0 \end{pmatrix}$$

Contributions

The joint 1 is revolut, the linear contr.  $J_{1L}$  is given by

$$J_{1L} = z_0 \times p_{0,e} = \begin{pmatrix} 0 & -1 & 0 \\ 1 & 0 & 0 \\ 0 & 0 & 0 \end{pmatrix} \begin{pmatrix} c_1 (a_4 c_2 c_4 + q_3 s_2) \\ s_1 (a_4 c_2 c_4 + q_3 s_2) \\ a_4 s_2 c_4 - q_3 c_2 \end{pmatrix} = \begin{pmatrix} -s_1 (a_4 c_2 c_4 + q_3 s_2) \\ c_1 (a_4 c_2 c_4 + q_3 s_2) \\ 0 \end{pmatrix}$$

$$J_{A1} = z_0 = \begin{pmatrix} 0 \\ 0 \\ 1 \end{pmatrix}$$

$$J_{L2} = S_1 p_{1,4} : \begin{pmatrix} 0 & 0 & -c_1 \\ 0 & 0 & -s_1 \\ c_1 & s_1 & 0 \end{pmatrix} \begin{pmatrix} c_1(z_4 c_{24} + q_3 s_2) \\ s_1(z_4 c_{24} + q_3 s_2) \\ z_4 s_{24} - q_3 c_2 \end{pmatrix} : \begin{pmatrix} c_1(q_3 c_2 - z_4 s_{24}) \\ s_1(q_3 c_2 - z_4 s_{24}) \\ z_4 c_{24} + q_3 s_2 \end{pmatrix}$$

$$J_{A2} = \begin{pmatrix} s_1 \\ -c_1 \\ 0 \end{pmatrix}$$

$$J_{L3} = \begin{pmatrix} c_1 s_2 \\ s_1 s_2 \\ -c_2 \end{pmatrix}$$

$$J_{A3} = 0$$

$$J_{L4} = \begin{pmatrix} 0 & 0 & -c_1 \\ 0 & 0 & -s_1 \\ c_1 & s_1 & 0 \end{pmatrix} \begin{pmatrix} c_1 z_4 c_{24} \\ s_1 z_4 c_{24} \\ z_4 s_{24} \end{pmatrix} = \begin{pmatrix} -z_4 c_1 s_{24} \\ -z_4 s_1 s_{24} \\ z_4 c_{24} \end{pmatrix}$$

$$J_{A4} = \begin{pmatrix} s_1 \\ -c_1 \\ 0 \end{pmatrix}$$

$$\Rightarrow J_L = \begin{bmatrix} -s_1(z_4 c_{24} + q_3 s_2) & c_1(q_3 c_2 - z_4 s_{24}) & c_1 s_2 & -z_4 c_1 s_{24} \\ c_1(z_4 c_{24} + q_3 s_2) & s_1(q_3 c_2 - z_4 s_{24}) & s_1 s_2 & -z_4 s_1 s_{24} \\ 0 & z_4 c_{24} + q_3 s_2 & -c_2 & z_4 c_{24} \end{bmatrix}$$

$$J_A = \begin{bmatrix} 0 & s_1 & 0 & s_1 \\ 0 & -c_1 & 0 & -c_1 \\ 1 & 0 & 0 & 0 \end{bmatrix}$$

We have 2 singular conf. if  $q_1=0$  and  $q_2=\pi/2$ , in such case, the second and fourth cols become lin. dependent:

$$J(q_1=0, q_2=\pi/2, q_3=0) = \begin{bmatrix} 0 & -z_4 s_{24} & 1 & -z_4 s_{24} \\ z_4 c_{24} & 0 & 0 & 0 \\ 0 & z_4 c_{24} & -1 & z_4 c_{24} \\ 0 & 0 & 0 & 0 \\ 0 & -1 & 0 & -1 \\ 1 & 0 & 0 & 0 \end{bmatrix} \quad \text{let } q_s = \begin{pmatrix} 0 \\ \pi/2 \\ 0 \\ -\pi/2 \end{pmatrix}$$

$$\Rightarrow J(q_s) = J_s = \begin{bmatrix} 0 & 0 & 1 & 0 \\ z_4 & 0 & 0 & 0 \\ 0 & z_4 & -1 & z_4 \\ 0 & 0 & 0 & 0 \\ 0 & -1 & 0 & -1 \\ 1 & 0 & 0 & 0 \end{bmatrix} \quad \text{I study Ker } J_s \text{ by solving } J_s \dot{q} = 0$$

The rank of  $J_s$  is 3, the max rank is 4.

$$\begin{bmatrix} 0 & 0 & 1 & 0 \\ 2_4 & 0 & 0 & 0 \\ 0 & 2_4 & -1 & 2_4 \\ 0 & 0 & 0 & 0 \\ 0 & -1 & 0 & -1 \\ 1 & 0 & 0 & 0 \end{bmatrix} \dot{q} \Rightarrow \begin{cases} \dot{q}_3 = 0 \\ 2_4 \dot{q}_1 = 0 \\ 2_4(\dot{q}_2 + \dot{q}_4) - \dot{q}_3 = 0 \\ -\dot{q}_2 - \dot{q}_4 = 0 \\ \dot{q}_1 = 0 \end{cases} \Rightarrow \begin{cases} \dot{q}_1 = 0 \\ \dot{q}_2 = -\dot{q}_4 \\ \dot{q}_3 = 0 \end{cases} \Rightarrow \text{a basis is } \text{Ker } J_s = \text{Span} \left\{ \begin{bmatrix} 0 \\ 1 \\ 0 \\ -1 \end{bmatrix} \right\}$$

The non realizable vectors are given by  $J_s^T x = 0$ :

$$\begin{pmatrix} 0 & 2_4 & 0 & 0 & 0 & 1 \\ 0 & 0 & 2_4 & 0 & -1 & 0 \\ 0 & 0 & -1 & 0 & 0 & 0 \\ 1 & 0 & 2_4 & 0 & -1 & 0 \end{pmatrix} x = 0 \Rightarrow \begin{cases} 2_4 x_2 + x_6 = 0 \\ 2_4 x_2 - x_5 = 0 \\ -x_3 = 0 \\ x_1 + 2_4 x_3 - x_5 = 0 \end{cases} \Rightarrow \begin{cases} x_6 = -2_4 x_2 \\ x_5 = 0 \\ x_3 = 0 \\ x_1 = 0 \end{cases} \Rightarrow \text{basis: } \begin{bmatrix} 0 \\ 1 \\ 0 \\ 0 \\ 0 \\ -2_4 \end{bmatrix}, \begin{bmatrix} 0 \\ 0 \\ 0 \\ 1 \\ 0 \\ 0 \end{bmatrix}$$

